wip: tactic support for transition proofs

Veil/Frontend/DSL/Action/Semantics/Definitions.lean
@@ -149,7 +149,8 @@ def VeilM.succeedsAndPreservesInvariantsAssuming (act : VeilM m ρ σ α) (assu 
 /-- The weakest precondition for an action that, given a precondition,
 _IF_ it succeeds (doesn't throw an exception), then it meets the
 post-condition. -/
-abbrev VeilM.meetsSpecificationIfSuccessful (act : VeilM m ρ σ α) (pre : SProp ρ σ) (post : RProp α ρ σ) : Prop :=
+@[reducible]
+def VeilM.meetsSpecificationIfSuccessful (act : VeilM m ρ σ α) (pre : SProp ρ σ) (post : RProp α ρ σ) : Prop :=
   [DemonSucc| triple pre act post]
 
 @[reducible]
@@ -162,7 +163,7 @@ def VeilM.meetsSpecificationIfSuccessfulAssuming (act : VeilM m ρ σ α) (assu 
 
 @[reducible]
 def VeilM.preservesInvariantsIfSuccessfulAssuming (act : VeilM m ρ σ α) (assu : ρ → Prop) (inv : SProp ρ σ) : Prop :=
-  VeilM.meetsSpecificationIfSuccessful act (fun th st => assu th ∧ inv th st) (fun _ => inv)
+  VeilM.meetsSpecificationIfSuccessfulAssuming act assu inv inv
 
 abbrev VeilM.choices (act : VeilM m ρ σ α) := ExtractNonDet WeakFindable act
 
@@ -185,11 +186,22 @@ def Transition.triple (act : Transition ρ σ) (pre : SProp ρ σ) (post : SProp
     act r₀ s₀ s₁ ->
     post r₀ s₁
 
-abbrev Transition.meetsSpecificationIfSuccessful (act : Transition ρ σ) (pre : SProp ρ σ) (post : SProp ρ σ) : Prop :=
+@[reducible]
+def Transition.meetsSpecificationIfSuccessful (act : Transition ρ σ) (pre : SProp ρ σ) (post : SProp ρ σ) : Prop :=
   Transition.triple act pre post
 
+@[reducible]
 def Transition.preservesInvariantsIfSuccesful (act : Transition ρ σ) (inv : SProp ρ σ) : Prop :=
   Transition.meetsSpecificationIfSuccessful act inv inv
+
+@[reducible]
+def Transition.meetsSpecificationIfSuccessfulAssuming (act : Transition ρ σ) (assu : ρ → Prop) (pre post : SProp ρ σ) : Prop :=
+  Transition.meetsSpecificationIfSuccessful act (fun th st => assu th ∧ pre th st) post
+
+@[reducible]
+def Transition.preservesInvariantsIfSuccessfulAssuming (act : Transition ρ σ) (assu : ρ → Prop) (inv : SProp ρ σ) : Prop :=
+  Transition.meetsSpecificationIfSuccessfulAssuming act assu inv inv
+
 
 end TransitionSemantics
 
